\section{Logical Symbols}
The logical symbols are a kind of symbols using for theoretical statements.
    \begin{table}[H]
        \centering
        \caption{Frequently-used Logical Symbols}
        \begin{tabular}{|c|c|}\hline
            Symbols&Meanings\\\hline
            $L\Longrightarrow P$& Proposition $L$ is contained in proposition $P$\\
            $L \Longleftrightarrow P $&Proposition $L$ is equivalent to proposition $P$\\
            $\lnot P$&Not $P$\\
            $L\wedge P$&Proposition $L$ and proposition $P$\\
            $L \vee P$&Proposition $L$ or proposition $P$\\
            \hline
        \end{tabular}
    \end{table}
e.g.\[((A\Longrightarrow B)\wedge(\lnot B)\Longrightarrow (\lnot A) )\]


stands for `` if $A$ is contained in  $B$,and $B$ is not true,then $A$ is not true''.

We also call $ A \Longleftrightarrow B$ ``$A$ is the necessary and suffiecent condition of $B$''.

The typical math proposition is like ``$A\Longrightarrow B$''.In order to prove this proposition ,we can use the  implication relationship \[A\Longrightarrow C_1\Longrightarrow \cdots \Longrightarrow C_n\Longrightarrow B\]The every implication relationship in this chain is general truth or proved proposition.

\begin{table}[H]
    \centering
    \caption{Truth Table}
    \begin{tabular}{|c|c|c|c|}
        \hline
        \multirow{2}{*}{$\lnot A$}                       & $A$                    & 0         & 1             \\ \cline{2-4} 
                                                 & $\lnot A$            & 1            & 0             \\ \hline
        \multirow{3}{*}{$A \vee B$}                       &       \diagbox{$A$}{$B$}     &    0        &       1        \\ \cline{2-4} 
                                                 &          0       &   0         &        1        \\ \cline{2-4} 
                                                 &       1         &  1        &        1       \\ \hline
        \multirow{3}{*}{$A \wedge B$}                       &        \diagbox{$A$}{$B$}    &           0&        1          \\ \cline{2-4} 
                                                 &     0         &     0          &      0          \\ \cline{2-4} 
                                                 &        1        &                0       &    1       \\ \hline
        \multirow{3}{*}{$A\Longrightarrow B$}                      &  \diagbox{$A$}{$B$} & 0  &  1 \\ \cline{2-4} 
                                                & 0  &  1 &  1 \\ \cline{2-4} 
                                                & 1  &  0 & 1  \\ \hline
        \end{tabular}
    \end{table}
\begin{question}$\lnot (A\wedge B )\Leftrightarrow (\lnot A \vee \lnot B)$.
\end{question}
\begin{proof}
    (Use the truth table)

    If $A$ is ture, $B$ is ture, $A\wedge B$ is ture. $\lnot (A\wedge B)$ is false.$\lnot A $ is false,$\lnot B$ is false, $(\lnot A \vee \lnot B)$ is false.

    If $A$ is ture, $B$ is false, $A\wedge B$ is false. $\lnot (A\wedge B)$ is true.$\lnot A $ is false,$\lnot B$ is true, $(\lnot A \vee \lnot B)$ is ture.

    If $A$ is flase, $B$ is true, $A\wedge B$ is false. $\lnot (A\wedge B)$ is true.$\lnot A $ is true,$\lnot B$ is false, $(\lnot A \vee \lnot B)$ is ture.

    If $A$ is false, $B$ is false, $A\wedge B$ is false. $\lnot (A\wedge B)$ is true.$\lnot A $ is true,$\lnot B$ is true, $(\lnot A \vee \lnot B)$ is ture.

    So
    \[\lnot (A\wedge B )\Leftrightarrow (\lnot A \vee \lnot B)\]
\end{proof}    

\begin{question}
    $(A \Rightarrow B)\Leftrightarrow\lnot A \vee B$.
\end{question}
\begin{proof}
    Firstly, we confirm the truth of \[(A \Rightarrow B)\Rightarrow\lnot A \vee B\]

    If $(A \Rightarrow B)$ is false, then $\lnot A \vee B$ is true.

    If $(A \Rightarrow B)$ is ture ,then we have two posibilities. The first is $A$ is ture, $B$ is true, so $\lnot A \vee B$ is true. The second is $A$ is false,then $B$ can be true or false, but $\lnot A \vee B$ will be true.

    Hence, $(A \Rightarrow B)\Rightarrow\lnot A \vee B$.

    Secondly, we prove \[(A \Rightarrow B)\Leftarrow\lnot A \vee B\]

    If $\lnot A \vee B$ is false, then $(A \Rightarrow B)$ is true.

    If $\lnot A \vee B$ is true, we have
    \begin{enumerate}
        \item $\lnot A$ is true, $B$ is false, then, $A$ is false, $(A \Rightarrow B)$ is true.
        \item $\lnot A$ is false, $B$ is true, then, $A$ is true, $(A \Rightarrow B)$ is true.
        \item $\lnot A$ is true, $B$ is true, then, $A$ is false, $(A \Rightarrow B)$ is true.
    \end{enumerate}

    So $(A \Rightarrow B)\Leftarrow\lnot A \vee B$.
\end{proof}

\begin{tips}
    
    \begin{enumerate}
        \item $\lnot(A\wedge B)\Leftrightarrow\lnot A\vee \lnot B$;
        \item $\lnot(A\vee B)\Leftrightarrow\lnot A\wedge \lnot B$;
        \item $(A\Rightarrow)\Leftrightarrow(\lnot B\Rightarrow\lnot A)$;
        \item $(A\Rightarrow)\Leftrightarrow(\lnot A\vee B)$;
        \item $\lnot(A\Rightarrow B)\Leftrightarrow A\wedge\lnot B$.
    \end{enumerate}
\end{tips}