\section{Normality, quotient groups, and homomorphisms}
\begin{ex}
    If $N$ is a subgroup of index 2 in a group $G$, then $N$ is normal in $G$.
\end{ex}

\begin{answer}
    $\forall a\in G\backslash N$, $G=N\cup Na=N\cup aN$ and $N\cap Na=\varnothing$, $N\cap aN=\varnothing$. So $\forall x\in Na$, $x\in G\backslash N\Rightarrow x\in aN$, $Na\subset aN$. Similarly, $aN\subset Na$, whence $Na=aN$, $N\lhd G$.
\end{answer}

$$ $$

\begin{ex}
    If $\{N_{i}|i\in I\}$ is a family of normal subgroups of a group $G$, then $\bigcap\limits_{i\in I}N_{i}$ is a normal subgroup of $G$.
\end{ex}

\begin{answer}
    $\bigcap\limits_{i\in I}N_{i}$ is a subgroup of $G$. $N_{i} (i\in I)$ are normal subgroups of $G$, so $\forall a\in G$, $aN_{i}a^{-1}=\{an_{i}a^{-1}|n_{i}\in N_{i}\}=N_{i}$. $\forall x=ana^{-1}\in a(\bigcap\limits_{i\in I}N_{i})a^{-1}$, $n\in N_{i}\Rightarrow x\in a(\bigcap\limits_{i\in I}N_{i})a^{-1}\subset \bigcap\limits_{i\in I}aN_{i}a^{-1}=\bigcap\limits_{i\in I}N_{i}$. $\bigcap\limits_{i\in I}N_{i}$ are normal subgroup of $G$.
\end{answer}

$$ $$

\begin{ex}
    Let $N$ be a subgroup of a group $G$. $N$ is normal in $G$ if and only if (right) congruence modulo $N$ is a congruence relation on $G$.
\end{ex}

\begin{answer}
    If $N\lhd G$. $\forall a,b\in G$, $ab^{-1}\in N\Leftrightarrow a^{-1}b\in N$. If $a_{1}\equiv b_{1}\mod N$, $a_{2}\equiv b_{2}\mod N$, then $a_{2}b_{2}^{-1}\in N$, $a_{1}N=Na_{1}=Nb_{1}\Rightarrow a_{1}Nb_{1}^{-1}=N$. So $a_{1}a_{2}b_{1}^{-1}b_{2}^{-1}=(a_{1}a_{2})(b_{1}b_{2})^{-1}\in N$. Similarly, $(a_{1}a_{2})^{-1}(b_{1}b_{2})\in N$. Congruence modulo $N$ is a congruence relation.

    If congruence modulo $N$ is a congruence relation. $\forall a_{1}\equiv b_{1}\mod N$, $a_{2}\equiv b_{2}\mod N$, we will have $a_{1}a_{2}\equiv b_{1}b_{2}\mod N$. Take $n\in N$ and fix $a_{2}\in G$, define $b_{2}=n^{-1}a_{2}$. Then $\forall n\in N$, $n$ can be expressed as $a_{2}b_{2}^{-1}$, $a_{2}\equiv b_{2}\mod N$. $\forall a_{1}\in G$ and $\forall b_{1}\equiv a_{1}\mod N$, $a_{1}nb_{1}^{-1}=a_{1}a_{2}b_{2}^{-1}b_{1}^{-1}\in N$. Take $b_{1}=a_{1}$ and $n$ varies in $N$, $a_{1}na_{1}^{-1}\in N\Rightarrow a_{1}Na_{1}^{-1}\subset N$. Thus $N\lhd G$.
\end{answer}

$$ $$

\begin{ex}
    Let $\sim$ be an equivalence relation on a group $G$ and let $N=\{a\in G |a\sim e\}$. Then $\sim$ is a congruence relation on $G$ if and only if $N$ is a normal subgroup of $G$ and $\sim$ is congruence modulo $N$.
\end{ex}

\begin{answer}
    If $G\lhd N$ and $\sim$ is congruence modulo $N$. $\forall a\in G$, $aNa^{-1}\subset N$. $\forall a_{1}, b_{1}, a_{2}, b_{2}\in G$, $a_{1}b_{1}^{-1}\in N$, $a_{2}b_{2}^{-1}\in N$. $a_{1}a_{2}(b_{1}b_{2})^{-1}=a_{1}a_{2}b_{2}^{-1}b_{1}^{-1}$, denote $n=a_{2}b_{2}^{-1}\in N$, $a_{1}a_{2}b_{2}^{-1}b_{1}^{-1}=a_{1}nb_{1}^{-1}\in a_{1}Nb_{1}^{-1}$. $\forall n\in N$, there exists $n'=b_{1}^{-1}a_{1}, n'\in N$ s.t. $a_{1}n=b_{1}n'$. So $a_{1}nb_{1}^{-1}=b_{1}n'b_{1}^{-1}\in b_{1}Nb_{1}^{-1}\subset N$. That means $(a_{1}a_{2})(b_{1}b_{2})^{-1}\in N$, $a\sim b$ is a congruence relation.

    If $a\sim b$ is a congruence relation. We first prove $N$ is a subgroup of $G$. $\forall a\in N$, $a\sim e$, $a^{-1}\sim a^{-1}\Rightarrow e\sim a^{-1}$, so $a^{-1}\sim e$, $a^{-1}\in N$. $\forall a,b \in N$, $b^{-1}\sim e$, $a\sim e\Rightarrow ab^{-1}\in e$, thus $N<G$.

    $\forall x\in G$, $xN=\{xa|a\sim e\}=\{xa|xa\sim xe\}=\{ax|ax\sim e\}=Nx$, so $N$ is normal in $G$. $x\sim y\Leftrightarrow y\in xN$. $\sim$ is congruence modulo $N$.
\end{answer}

$$ $$

\begin{ex}
    Let $N<S_{4}$ consist of all those permutations $\sigma$ such that $\sigma(4)=4$. Is $N$ normal in $S_{4}$?
\end{ex}

\begin{answer}
    $N=\{(1),(12),(13),(23),(123),(132)\}$. Take $a=(14)\in G$, $a^{-1}=(14)$, $a^{-1}(12)a=(24)\notin N$. So $N$ is not normal in $S_{4}$.
\end{answer}

$$ $$

\begin{ex}
    Let $H<G$; then the set $aHa^{-1}$ is a subgroup for each $a\in G$, and $H\cong aHa^{-1}$. 
\end{ex}

\begin{answer}
    $H<G$, $aHa^{-1}=\{aha^{-1}|h\in H\}$. $\forall x,y\in aHa^{-1}$, $x=ah_{1}a^{-1}$, $y=ah_{2}a^{-1}$. $y^{-1}=ah_{2}^{-1}a^{-1}$, $xy=ah_{1}h_{2}^{-1}a^{-1}\in aHa^{-1}$, so $aHa^{-1}< G$.

     Take $f: H\to aHa^{-1}$ as $f(h)=aha^{-1}$. If $f(h_{1})=f(h_{2})=ah_{1}a^{-1}=ah_{2}a^{-1}$, then $h_{1}=h_{2}$, so $f$ is an injection. $f$ is a surjection because $\forall x\in aHa^{-1}$, $f(a^{-1}xa)=x$, $a^{-1}xa\in H$. In conclusion, $H\cong aHa^{-1}$.
\end{answer}

$$ $$

\begin{ex}
    Let $G$ be a finite group and $H$ a subgroup of $G$ of order $n$. If $H$ is the only subgroup of $G$ of order $n$, then $H$ is normal in $G$.
\end{ex}

\begin{answer}
    Applying \textbf{Exercise 1.5.6}, $\forall a\in G$, $aHa^{-1}\cong H$. $\left| aHa^{-1} \right| =\left| H \right| =n\Rightarrow aHa^{-1}=H$. Whence $H\lhd G$.
\end{answer}

$$ $$

\begin{ex}
    All subgroups of the quaternion group are normal.
\end{ex}

\begin{answer}
    $Q_{8}=\{a,b,a^{2},ba,ab,a^{2}b,ab^{2},a^{2}b^{2}\}$ where $a^{2}=b^{2}$, $a_{1}b=ba=a^{3}b$ and $\left| a \right| =\left| b \right| =4$. There are several subgroups $\{a,a^{2},ab^{2},a^{2}b^{2}\}$, $\{b, a^{2}, a^{2}b,\\ a^{2}b^{2}\}$, $\{ab,a^{2}b^{2}\}$, $\{ba,a^{2}b^{2}\}$, $\{a^{2},a^{2}b^{2}\}$. From \textbf{Exercise 1.5.1}, we know the first two subgroups are normal in $G$. For $\{ab,a^{2}b^{2}\}$, $\{ba,a^{2}b^{2}\}$, $\{a^{2},a^{2}b^{2}\}$, we can check that $ab, ba, a^{2}$ is communicative in $G$, that is $\forall x\in G$, $xabx^{-1}=ab$, $xbax^{-1}=ba$, $xa^{2}x^{-1}=a^{2}$. They are all normal in $G$.
\end{answer}

$$ $$

\begin{ex}
    \begin{enumerate}[(a)]
        \item If $G$ is a group, then the center of $G$ is a normal subgroup of $G$;
        \item the center of $S_{n}$ is the identity subgroup for all $n>2$.
    \end{enumerate}
\end{ex}

\begin{answer}
    \begin{enumerate}[(a)]
        \item By the definition of center $C$, $\forall x\in G$ and $a\in C$, $ax=xa$, so $xCx^{-1}=C$. $C$ is normal in $G$.
        \item $\forall x\in S_{n}$, $x$ can be expressed as \[x=(a_{1}a_{2}\cdots a_{i_{1}})(a_{i_{1}+1}a_{i_{1}+2}\cdots a_{i_{2}})\cdots(a_{i_{n-1}+1}a_{i_{n-1}+2}\cdots a_{i_{n}})\]
        Those cycles $(a_{1}a_{2}\cdots a_{i_{1}})$, $(a_{i_{1}+1}a_{i_{1}+2}\cdots a_{i_{2}})$, \dots, $(a_{i_{n-1}+1}a_{i_{n-1}+2}\cdots a_{i_{n}})$ are all disjoint, so they are communicative.

        If there exists cycles whose length is longer than 2. WLOG, assume $i_{1}>2$. Take $y=(a_{1}a_{2})$, \[y^{-1}xy=(a_{1}a_{2})(a_{1}a_{2}\cdots a_{i_{1}})(a_{1}a_{2})\cdots(a_{i_{n-1}+1}a_{i_{n-1}+2}\cdots a_{i_{n}})\] $(a_{1}a_{2})(a_{1}a_{2}\cdots a_{i_{i}})(a_{1}a_{2})=(a_{2}a_{1}a_{3}\cdots a_{i_{1}})$, so $y^{-1}xy\neq x$, $x\notin C$. 

        If $x=(a_{1}a_{2})(a_{3}a_{4})\cdots(a_{2n-1}a_{2n})$ and $n\geq 2$. Take $y=(a_{1}a_{3})$, \[\begin{aligned}
            y^{-1}xy&=(a_{1}a_{3})(a_{1}a_{2})(a_{3}a_{4})\cdots(a_{2n-1}a_{2n})(a_{1}a_{3})\\&=(a_{1}a_{3})(a_{1}a_{2})(a_{3}a_{4})(a_{1}a_{3})\cdots(a_{2n-1}a_{2n})\\&=(a_{1}a_{4})(a_{2}a_{3})\cdots(a_{2n-1}a_{2n})\\&\neq x
        \end{aligned}\] So $x\notin C$.

        If $x=(a_{1}a_{2})$. Take $y=(a_{1}a_{3})$, $y^{-1}xy=(a_{2}a_{3})\neq x$, so $x\notin C$.

        In conclusion, $C=\{(1)\}$.
    \end{enumerate}
\end{answer}

$$ $$

\begin{ex}
    Find subgroups $H$ and $K$ of $D_{4}^{*}$ such that $H\lhd K$ and $K\lhd D_{4}^{*}$, but $H$ is not normal in $D_{4}^{*}$.
\end{ex}

\begin{answer}
    $D_{4}^{*}=\{I,R,R^{2},R^{3},T_{x},T_{y},T_{13},T_{24}\}$. Take $K=\{I, R, T_{x}, T_{y}\}$, $H=\{I, T_{x}\}$. We can easily verify that $H\lhd K$ and $K\lhd  D_{4}^{*}$ but $K\ntriangleleft  D_{4}^{*}$.
\end{answer}

$$ $$

\begin{ex}
    If $H$ is a cyclic subgroup of a group $G$ and $H$ is normal in $G$, then every subgroup of $H$ is normal in $G$.
\end{ex}

\begin{answer}
    Assume $K<H\lhd G$, $H$ has the generator $a$, and $K$ has the generator $a^{n}$. Here we used: \emph{Every subgroup of a cyclic group is cyclic.} This can be easily proved by the conclusion $H\cong Z_{m}$ for some $m\in \mathbf{Z}$. $\forall x\in G$, $h=a^{s}\in H$, $x^{-1}a^{s}x=a^{t}\in H$. Assume $x^{-1}ax=a^{m}$, then $x^{-1}a^{n}x=(x^{-1}ax)^{n}=a^{mn}=a^{k}$, so $n|k$, $a^{k}\in K$. $x^{-1}Kx\subset K$, $K$ is normal in $G$.
\end{answer}

$$ $$

\begin{ex}
    If $H$ is a normal subgroup of a group $G$ such that $H$ and $G/H$ are finitely generated, then so is $G$.
\end{ex}

\begin{answer}
    Assume $A=\{a_{1},a_{2},\dots, a_{m}\}$, $B=\{b_{1}, b_{2},\dots, b_{n}\}$. $H=\left\langle A\right\rangle$, $G /H=\left\langle \{Hb_{i}|b_{i}\in B\}\right\rangle$. We prove that $G$ can be generated by $A\cup B$. $\forall x\in G$, $x$ is in one of the right cosets of $H$, $x\in Ha$. $Ha\in G /H$ so $Ha=\prod\limits_{b_{i}\in B}Hb_{i}^{s_{i}}=H(\prod\limits_{b_{i}\in B}b_{i}^{s_{i}})$. Thus $a^{-1}(\prod\limits_{b_{i}\in B}b_{i}^{s_{i}})=a'\in H$. $H$ is generated by $A$ so $xa^{-1}=\prod\limits_{a_{i}\in A}a_{i}^{t_{i}}$, $a'=\prod\limits_{a_{i}\in A}a_{i}^{-r_{i}}$. Then \[x=(\prod\limits_{a_{i}\in A}a_{i}^{t_{i}+r_{i}})(\prod\limits_{b_{i}\in B}b_{i}^{s_{i}})\in\left\langle A\cup B\right\rangle\] Thus $G\subset\left\langle A\cup B\right\rangle$ is finitely generated.
\end{answer}

$$ $$

\begin{ex}
    \begin{enumerate}[(a)]
        \item Let $H\lhd G$, $K\lhd G$. Show that $H\vee K$ is normal in $G$.
        \item Prove that the set of all normal subgroups of $G$ forms a complete lattice under inclusion.
    \end{enumerate}
\end{ex}

\begin{answer}
    \begin{enumerate}[(a)]
        \item $\forall x\in G$, $a\in H\vee K$, we need to prove $x^{-1}ax\in H\vee K$. $a\in H\vee K$ so $a$ can be expressed  as \[a=b_{1}^{n_{1}}b_{2}^{n_{2}}\cdots b_{t}^{n_{t}}\quad \text{where } b_{i}\in H \text{ or } b_{i}\in K, i=1,2,\dots,t\] so $x^{-1}ax= x^{-1}b_{1}^{n_{1}}\cdots b_{t}^{n_{t}}x =(x^{-1}b_{1}x)^{n_{1}}(x^{-1}b_{2}x)^{n_{2}}\cdots (x^{-1}b_{t}x)^{n_{t}}$.\\ $H\lhd G$, $K\lhd G$, so $x^{-1}b_{i}x\in H\vee K, i=1,2,\dots,t$ and \[x^{-1}ax=(x^{-1}b_{1}x)^{n_{1}}(x^{-1}b_{2}x)^{n_{2}}\cdots (x^{-1}b_{t}x)^{n_{t}}\in H\vee K\] $H\vee K\lhd G$.
        \item Actually, in \textbf{Exercise 1.2.19} and (a), we have proved lub exists.
        
        Now we only consider glb. For $H\lhd G$, $K\lhd G$. If $H\cap K\lhd G$, then their glb is $H\cap K$. If not, assume there exists $A<H\cap K$, $B<H\cap K$, $A$, $B$ are both normal in $H$ and $K$. And there doesn't exists $I$ s.t. $A\lhd I\lhd H$, $A\lhd I\lhd K$, $B\lhd I\lhd H$, $B\lhd I\lhd K$. Just like the figure:
        
        \begin{figure}[H]\centering
            \begin{tikzpicture}[scale=0.9]
                \node [above] at (0,0) {$A$};
                \node [above] at (0,2) {$H$};
                \node [above] at (2,2) {$K$};
                \node [above] at (2,0) {$B$};
                \draw [-] (1.9,2) to (0.1,0.5);
                \draw [-] (2,2) to (2,0.5);
                \draw [-] (0,2) to (0,0.5);
                \draw [-] (0.1,2) to (1.9,0.5);
            \end{tikzpicture}
        \end{figure}
        But $A<H\cap K$, $B<H\cap K\Rightarrow A\vee B<H\cap K$. So $A\vee B\lhd H$, $A\vee B\lhd K$. That's contradictory! There is only one lower bound for $\{H,K\}$. Notice that $\{e\}<H\cap K$ so there exists at least one subgroup satisfies the condition. We have proved normality forms a lattice.
    \end{enumerate}
\end{answer}

$$ $$

\begin{ex}
    If $N_{1}\lhd G_{1}$, $N_{2}\lhd G_{2}$ then $(N_{1}\times N_{2})\lhd (G_{1}\times G_{2})$ and $(G_{1}\times G_{2})/(N_{1}\times N_{2})\cong (G_{1}/N_{1})\times(G_{2}/N_{2})$.
\end{ex}

\begin{answer}
    Take $a\in (N_{1}\times N_{2})$, $a=(n_{1},n_{2})$ where $n_{1}\in N_{1}$, $n_{2}\in N_{2}$. $\forall x\in (G_{1}\times G_{2})$, $x=(g_{1},g_{2})$ where $g_{1}\in G_{1}$, $g_{2}\in G_{2}$. $x^{-1}=(g_{1}^{-1},g_{2}^{-1})$, $x^{-1}ax=(g_{1}^{-1}n_{1}g_{1},g_{2}^{-1}n_{2}g_{2})$. $N_{1}\lhd G_{1}$, $N_{2}\lhd G_{2}$, so $g_{1}^{-1}n_{1}g_{1}\in N_{1}$, $g_{2}^{-1}n_{2}g_{2}\in N_{2}$. $x^{-1}ax\in (N_{1}\times N_{2})$. Thus $(N_{1}\times N_{2})\lhd (G_{1}\times G_{2})$.

    Assume $G_{1}=\bigcup\limits_{i\in I}N_{1}a_{i}$, $G_{2}=\bigcup\limits_{j\in J}N_{2}b_{j}$. Then $G_{1}\times G_{2}=\bigcup\limits_{i\in I}N_{1}a_{i}\times \bigcup\limits_{j\in J}N_{2}b_{j}$. Denote $A=\{a_{i}|i\in I\}$, $B=\{b_{j}|j\in J\}$. We construct two bijections $(G_{1}\times G_{2})/(N_{1}\times N_{2})\to A\times B$ and $(G_{1}/N_{1})\times(G_{2}/N_{2})$.\[f: N_{1}a_{i}\times N_{2}b_{j}\mapsto (a_{i},b_{j})\]\[g: (N_{1}a_{i}, N_{2}b_{j})\mapsto (a_{i},b_{j})\] Take $h=g^{-1}\circ f$, $f,g$ are bijections, so $h$ is an isomorphism. $(G_{1}\times G_{2})/(N_{1}\times N_{2})\cong (G_{1}/N_{1})\times(G_{2}/N_{2})$.
\end{answer}

$$ $$

\begin{ex}
    Let $N\lhd G$ and $K\lhd G$. If $N\cap K=\left\langle e\right\rangle$ and $N\vee K=G$, then $G/N\cong K$.
\end{ex}

\begin{answer}
    Assume $G=\bigcup\limits_{i\in I}Na_{i}$, we construct $f:k \to G /N$. We prove that $\forall x,y\in K$, $x,y$ belong to different cosets of $N$. Suppose not. $\exists x,y \in K$, $x,y\in Na_{i}$, then $xy^{-1}\in N\Rightarrow x=y$. That's contradictory! So $f$ is a monomorphism.

    $G=H\vee K$, so $G=HK$. we can write $x$ as $pq$, where $p\in H$, $q\in K$. $\left| G/H \right|=\left[G:H\right]=\left[HK:H\right]=\left[K:K\cap H\right]=\left| K \right| $. $f$ is a epimorphism.
    
    Thus, $G /N\cong K$.
\end{answer}

$$ $$

\begin{ex}
    If $f:G\to H$ is a homomorphism, $H$ is abelian and $N$ is a subgroup of $G$ containing $\mathrm{Ker}f$, then $N$ is normal in $G$.
\end{ex}

\begin{answer}
    Assume there exists $x\in G$, $x\notin N$ s.t. $f(x)\in f(N)$. $\exists n\in N$, $f(x)=f(n)$, $f(xn^{-1})=f(x)f(n)^{-1}=e'\Rightarrow xn^{-1}\in\mathrm{Ker}f\Rightarrow x\in N$. That's contradictory! $\forall x\in G$, $n\in N$, $f(x^{-1}nx)=f(x^{-1})f(n)f(x)=f(n)\in f(N)$, so $x^{-1}nx\in N$. Thus, $N\lhd G$.
\end{answer}

$$ $$

\begin{ex}
    \begin{enumerate}[(a)]
        \item Consider the subgroups $\left\langle 6\right\rangle$ and $\left\langle 30\right\rangle$ of $\mathbf{Z}$ and show that $\left\langle 6\right\rangle /\left\langle 30\right\rangle\cong Z_{5}$.
        \item For any $k,m>0$, $\left\langle k\right\rangle /\left\langle km\right\rangle\cong Z_{m}$; in particular, $\mathbf{Z}/\left\langle m\right\rangle=\left\langle 1\right\rangle /\left\langle m\right\rangle\cong Z_{m}$.
    \end{enumerate}
\end{ex}

\begin{answer}
    \begin{enumerate}[(a)]
        \item $\left\langle 6\right\rangle=\{6n|n\in \mathbf{Z}\}$, $\left\langle 30\right\rangle=\{30n|n\in \mathbf{Z}\}$. So $\left\langle 6\right\rangle/\left\langle 30\right\rangle=\{\left\langle 30\right\rangle, \left\langle 30\right\rangle +6, \left\langle 30\right\rangle +12, \left\langle 30\right\rangle +18, \left\langle 30\right\rangle +24\}\cong Z_{5}$
        \item $\left\langle km\right\rangle\lhd \left\langle k\right\rangle$, $\left\langle k\right\rangle=\bigcup\limits_{i\in I}(\left\langle km\right\rangle +a_{i})$. For $x\in \left\langle k\right\rangle$, $x\equiv a_{i}\mod km$, then $x\in \left\langle km \right\rangle +a_{i}$. $f:\left\langle k\right\rangle/\left\langle km\right\rangle\to \{a_{i}|i\in I\}$ defined by $f(\left\langle km\right\rangle +a_{i})=a_{i}$ is a bijection. We check that $g: \{a_{i}|i\in I\}\to Z_{m}$ is also a bijection. Define $b_{i}\equiv \frac{a_{i}}{k}\mod m$, $g(a_{i})=b_{i}$. If there exists $b_{i}=b_{j}$ for $i\neq j$, $a_{i}\equiv a_{j}\mod km$. That's contradictory! So $g$ is an injection. $g$ is obviously a surjection, so $g$ is a bijection. Take $h= g\circ f:\left\langle k\right\rangle /\left\langle km \right\rangle\to Z_{m}$ is a isomorphism, so $\left\langle k\right\rangle /\left\langle km \right\rangle\cong Z_{m}$.
    \end{enumerate}
\end{answer}

$$ $$

\begin{ex}
    If $f: G \to H$ is a homomorphism with kernel $N$ and $K<G$, then prove that $f^{-1}(f(K))=KN$. Hence $f^{-1}(f(K))=K$ if and only if $N<K$.
\end{ex}

\begin{answer}
    Take $x\in f^{-1}(f(K))$, then there exists $k\in K$ s.t. $f(x)=f(k)$. $f(xk^{-1})=f(x)f(k)^{-1}=e'\in f(K) \Rightarrow xk^{-1}\in\mathrm{Ker}f=N$. Thus, $x\in Nk\subset NK$, $f^{-1}(f(K))\subset NK$.

    $\forall x=nk\in NK$, where $n\in N$ and $k\in K$. $f(x)=f(n)f(k)=e'f(k)\in f(K)$, so $NK\subset f^{-1}(f(K))$.

    Thus, $f^{-1}(f(K))=NK$. Hence $f^{-1}(f(K))=K$ if and only if $N<K$.
\end{answer}

$$ $$

\begin{ex}
    If $N\lhd G$, $\left[G:H\right]$ finite, $H<G$, $\left| H \right| $ finite, and $\left[G:N\right]$ and $\left| H \right| $ are relatively prime, then $H<N$.
\end{ex}

\begin{answer}
    $N\lhd G\Rightarrow NH<G$. By the second isomorphism theorem, $NH /N\cong H/H\cap N\Rightarrow \left[NH:N\right]=\left[H:H\cap N\right]$. Assume $\left[G:N\right]=m$, $\left| H \right| =n$, $\left| G \right| =mnp$ where $(m,n)=1$. Then $\left| N \right| =np$, $N<NH$, assume $\left| NH \right| =knp$, $NH<G\Rightarrow knp|mnp\Rightarrow k|m$. $\left[NH:N\right]=\left[H:H\cap N\right]=k\Rightarrow k|n$. So $k=1$, $NH=N$ which means $H<N$.
\end{answer}

$$ $$

\begin{ex}
    If $N\lhd G$, $\left| N \right|$ finite, $H<G$, $\left[G:N\right] $ finite, and $\left[G:H\right]$ and $\left| N \right| $ are relatively prime, then $N<H$.
\end{ex}

\begin{answer}
    $N\lhd G\Rightarrow NH<G$. By the second isomorphism theorem, $NH /N\cong H/H\cap N\Rightarrow \left[NH:N\right]=\left[H:H\cap N\right]$. Assume $\left[G:H\right]=m$, $\left| N \right| =n$, $\left| G \right| =mnp$ where $(m,n)=1$. Then $\left| H \right| =np$, $H<NH$, assume $\left| NH \right| =knp$, $NH<G\Rightarrow knp|mnp\Rightarrow k|m$. $\left[NH:N\right]=\left[H:H\cap N\right]=kp\Rightarrow kp|np\Rightarrow k|n$. So $k=1$, $NH=H$ which means $N<H$.
\end{answer}

$$ $$

\begin{ex}
    If $H$ is a subgroup of $Z(p^{\infty})$ and $H\neq Z(p^{\infty})$, then $Z(p^{\infty}) /H\cong Z(p^{\infty})$.
\end{ex}

\begin{answer}
    From \textbf{Exercise 1.3.7}(b), we know that $H$ has the form $\left\langle \bar{\frac{1}{p^{n}}}\right\rangle$. Take $x_{i}=\bar{\frac{1}{p^{n+i}}}+H$, $x_{1}=\bar{\frac{1}{p^{n+1}}}+H$. \[\sum_{m=1}^{p}x_{1}=\bar{\frac{p}{p^{n+1}}}+pH=\bar{\frac{1}{p^{n}}}+H=H\] \[\sum_{m=1}^{p}x_{i}=\bar{\frac{p}{p^{n+i}}}+pH=\bar{\frac{1}{p^{n+i-1}}}+H=x_{i-1}\] Take $A=\{x_{i}|i\in \mathbf{Z}_{+}\}$, $\left\langle A\right\rangle\cong Z(p^{\infty})$ by \textbf{Exercise 1.3.7}(e). $\forall x\in \left\langle A\right\rangle$, $x\in Z(p^{\infty}) /H$, so $\left\langle A\right\rangle\subset Z(p^{\infty}) /H$. Take $x\in Z(p^{\infty}) /H$, $x=y+H$ where $y=\sum\limits_{i=1}^{m}\frac{a_{i}}{p^{n+i}}$, $x=\sum\limits_{i=1}^{m}(\frac{a_{i}}{p^{n+i}}+H)\in \left\langle A\right\rangle$. Thus, $Z(p^{\infty}) /H\subset \left\langle A\right\rangle$, $\left\langle A\right\rangle=Z(p^{\infty}) /H\cong Z(p^{\infty})$.
\end{answer}